src/Narcissus/BaseFormats.v
@@ -1,10 +1,10 @@
 Require Export
         Fiat.Narcissus.Formats.Base.FMapFormat
         Fiat.Narcissus.Formats.Base.UnionFormat
-        (* Fiat.Narcissus.Formats.Base.SequenceFormat *)
-        (* Fiat.Narcissus.Formats.Base.StrictTerminalFormat *)
-        (* Fiat.Narcissus.Formats.Base.LaxTerminalFormat *)
-        (* Fiat.Narcissus.Formats.Base.FixFormat *)
+        Fiat.Narcissus.Formats.Base.SequenceFormat
+        Fiat.Narcissus.Formats.Base.StrictTerminalFormat
+        Fiat.Narcissus.Formats.Base.LaxTerminalFormat
+        Fiat.Narcissus.Formats.Base.FixFormat
         (* Fiat.Narcissus.Formats.Base.EnqueueFormat *)
         .
 
